Added cli messages. Added reflex patterns.

gen/su/nsk/iae/reflex/antlr/ReflexVisitor.java
@@ -1,7 +1,7 @@
 // Generated from C:/Users/iarte/IdeaProjects/ReflexVCG/src/main/java/su/nsk/iae/reflex/antlr/Reflex.g4 by ANTLR 4.13.1
 package su.nsk.iae.reflex.antlr;
 import org.antlr.v4.runtime.tree.ParseTreeVisitor;
-import su.nsk.iae.reflex.antlr.ReflexParser;
+
 /**
  * This interface defines a complete generic visitor for a parse tree produced
  * by {@link ReflexParser}.
