reflex case stadies/RevolvingDoor/RevolvingDoor_VC3.thy
@@ -2,13 +2,265 @@ theory RevolvingDoor_VC3
 imports RevolvingDoorTheory
 begin
 
-lemma
- assumes base_inv:"(inv st0)"
- and st1:"(st1=(setVarBool st0 ''inp_2'' inp_2))"
- and st2:"(st2=(setVarBool st1 ''inp_1'' inp_1))"
+
+definition extra1_1_Q1 :: "state\<Rightarrow>bool" where 
+"extra1_1_Q1 x \<equiv> True \<longrightarrow> getPstate x ''Controller'' =''motionless''"
+
+lemma extra1_1_Q1_to_extra1_Q1:
+  "getPstate s ''Controller'' = ''motionless'' \<and> P1 extra1_1_Q1 s \<Longrightarrow> extra1_Q1 s"
+  using extra1_1_Q1_def extra1_Q1_def P1_def apply auto
+  done
+
+definition extra1_2_Q2 ::"state\<Rightarrow>state\<Rightarrow>state\<Rightarrow>bool" where
+"extra1_2_Q2 s s3 s2 \<equiv>
+      toEnvNum s2 s3 = 1 \<and>
+       getPstate s2 ''Controller'' = ''rotating'' \<and>
+       1000 \<le> ltime s2 ''Controller'' \<and>
+       \<not> getVarBool s3 ''user'' \<and>
+       \<not> getVarBool s3 ''pressure'' \<and>
+       (\<forall>s4 s5.
+           toEnvP s4 \<and>
+           toEnvP s5 \<and>
+           substate s3 s4 \<and>
+           substate s4 s5 \<and>
+           substate s5 s \<and> toEnvNum s4 s5 = 1 \<longrightarrow>
+           getPstate s4 ''Controller'' = ''motionless'' \<and>
+           \<not> getVarBool s5 ''user'')"
+(*
+lemma extra1_2_Q2_to_extra1_Q1:
+"getPstate s ''Controller'' = ''motionless'' \<and> PE2 extra1_2_Q2 s \<Longrightarrow> extra1_Q1 s" 
+  using extra1_2_Q2_def extra1_Q1_def PE2_def apply simp
+  apply (rule uncurry)
+    apply auto
+  apply 
+  done*)
+find_theorems "(_\<longrightarrow>_\<longrightarrow>_) \<Longrightarrow> (_\<and>_\<longrightarrow>_)"
+lemma extra:
+ assumes base_inv:"(extraInv st0)"
+ and st1:"(st1=(setVarBool st0 ''pressure'' pressure))"
+ and st2:"(st2=(setVarBool st1 ''user'' user))"
  and st2_Controller_state:"(getPstate st2 ''Controller'')=''motionless''"
- and st2_if3:"(getVarBool st2 ''inp_1'')=False"
+ and st2_if3:"(getVarBool st2 ''user'')=False"
  and st3:"(st3=(toEnv st2))"
-shows "(inv st3)"
+ and st_final:"(st_final=st3)"
+shows "(extraInv st_final)" 
+proof (simp only: extraInv_def;intro conjI)
+  show "toEnvP st_final" using assms by auto
+next
+  show "extraControllerStates st_final"
+  proof -
+    have "extraControllerStates st0" using extraInv_def base_inv by blast
+    then show ?thesis using assms extraControllerStates_def by auto
+  qed
+next
+  show "extraMotionlessOut st_final" 
+  proof (simp only: extraMotionlessOut_def; rule allI; rule impI)
+    fix s1
+    assume prems:"toEnvP s1 \<and>
+          substate s1 st_final \<and>
+          getPstate s1 ''Controller'' = ''motionless''"
+    then show "\<not> getVarBool s1 ''rotation'' \<and>
+                \<not> getVarBool s1 ''brake''"
+    proof (cases)
+      assume 1:"s1=st_final"
+      have "getPstate st0 ''Controller'' = ''motionless''" using assms by simp
+      moreover have "extraMotionlessOut st0" using base_inv extraInv_def by blast
+      ultimately have buff:"\<not> getVarBool st0 ''rotation'' \<and> \<not> getVarBool st0 ''brake''" using base_inv extraInv_def extraMotionlessOut_def substate_refl by blast
+      then have 2:"\<not> getVarBool st_final ''rotation''" using assms by auto
+      have 3:"\<not> getVarBool st_final ''brake''" using assms buff by auto
+      show  ?thesis using 1 2 3  by auto
+    next
+      assume 1:"s1\<noteq>st_final"
+      have "predEnv st_final = st0" using assms extraInv_def by auto
+      then have 2:"substate s1 st0" using 1 assms prems substate_eq_or_predEnv by blast 
+      have "extraMotionlessOut st0" using base_inv extraInv_def by auto
+      thus ?thesis using 1 2 prems assms extraInv_def extraMotionlessOut_def[of st0] substate_refl by blast
+    qed
+  qed
+next
+  show "extraRotatingOut st_final" 
+  proof -
+    have "extraRotatingOut st0" using extraInv_def base_inv by blast
+    then show ?thesis using assms extraRotatingOut_def by auto
+  qed
+next
+  show "extraSuspendedOut st_final"
+  proof -
+    have "extraSuspendedOut st0" using extraInv_def base_inv by blast
+    then show ?thesis using assms extraSuspendedOut_def by auto
+  qed     
+next
+  show "extra2 st_final"
+  proof -
+    have "extra2 st0" using base_inv extraInv_def by auto
+    thus ?thesis using assms extra2_def by auto
+  qed
+next
+  show "extra3 st_final"
+  proof -
+    have "extra3 st0" using base_inv extraInv_def by auto
+    thus ?thesis using assms extra3_def by auto
+  qed
+next
+  show "extra6 st_final"
+  proof -
+    have "extra6 st0" using base_inv extraInv_def by auto
+    thus ?thesis using assms extra6_def by auto
+  qed
+next
+  show "extra4 st_final"
+  proof -
+    have "extra4 st0" using base_inv extraInv_def by auto
+    thus ?thesis using assms extra4_def by auto
+  qed
+next
+  show "extra5 st_final" 
+  proof -
+    have "extra5 st0" using base_inv extraInv_def by auto
+    thus ?thesis using assms extra5_def by auto
+  qed
+next
+  show "extra7 st_final"
+  proof -
+    have "extra7 st0" using base_inv extraInv_def by auto
+    thus ?thesis using assms extra7_def by auto
+  qed
+next
+  show "extra1 st_final"
+  proof -
+    have "toEnvP st0 \<and> toEnvP st_final \<and> st0 = predEnv st_final" using assms extraInv_def by auto
+    moreover have "P1 extra1_Q1 st0" using P1_extra1_Q1_st0 base_inv extraInv_def by auto
+    moreover have "extra1_Q1 st_final" 
+    proof -
+      have "extra1_Q1 st0" using assms extraInv_def using P1_def calculation(2) substate_refl by blast
+      then have "(\<forall> s2.
+      toEnvP s2 \<and>
+      substate s2 st0 \<longrightarrow>
+      getPstate s2 ''Controller'' = ''motionless'')\<or>
+    (\<exists> s2 s3.
+      toEnvP s2 \<and>
+      toEnvP s3 \<and>
+      substate s2 s3 \<and>
+      substate s3 st0 \<and>
+      toEnvNum s2 s3 = 1 \<and>
+      getPstate s2 ''Controller'' = ''rotating'' \<and>
+      ltime s2 ''Controller'' \<ge> 1000 \<and>
+      \<not> getVarBool s3 ''user'' \<and>
+      \<not> getVarBool s3 ''pressure'' \<and>
+      (\<forall> s4 s5.
+        toEnvP s4 \<and> 
+        toEnvP s5 \<and> 
+        substate s3 s4 \<and> 
+        substate s4 s5 \<and> 
+        substate s5 st0 \<and>
+        toEnvNum s4 s5 = 1 \<longrightarrow>
+          getPstate s4 ''Controller'' = ''motionless'' \<and>
+          \<not> getVarBool s5 ''user''))" using extra1_Q1_def assms by auto
+      then show ?thesis 
+      proof (rule disjE)
+        assume "\<forall>s2. 
+                  toEnvP s2 \<and>
+                  substate s2 st0 \<longrightarrow>
+                 getPstate s2 ''Controller'' =''motionless''"
+        then have "P1 extra1_1_Q1 st0" using P1_def extra1_1_Q1_def by auto
+        moreover have "toEnvP st0 \<and> toEnvP st_final \<and> st0 = predEnv st_final" using assms extraInv_def by auto
+        moreover have "extra1_1_Q1 st_final" by (simp add: extra1_1_Q1_def st2_Controller_state st3 st_final)
+        ultimately have "P1 extra1_1_Q1 st_final" using one_pos_cond by auto
+        then show ?thesis using P1_def extra1_1_Q1_def 
+          by (simp add: extra1_1_Q1_to_extra1_Q1 st2_Controller_state st3 st_final)
+      next
+        assume "\<exists>s2 s3.
+       toEnvP s2 \<and>
+       toEnvP s3 \<and>
+       substate s2 s3 \<and>
+       substate s3 st0 \<and>
+       toEnvNum s2 s3 = 1 \<and>
+       getPstate s2 ''Controller'' = ''rotating'' \<and>
+       1000 \<le> ltime s2 ''Controller'' \<and>
+       \<not> getVarBool s3 ''user'' \<and>
+       \<not> getVarBool s3 ''pressure'' \<and>
+       (\<forall>s4 s5.
+           toEnvP s4 \<and>
+           toEnvP s5 \<and>
+           substate s3 s4 \<and>
+           substate s4 s5 \<and>
+           substate s5 st0 \<and> toEnvNum s4 s5 = 1 \<longrightarrow>
+           getPstate s4 ''Controller'' = ''motionless'' \<and>
+           \<not> getVarBool s5 ''user'')"
+        then show ?thesis by sorry
+    qed
+  qed
+  thus ?thesis by sorry
+  qed
+
+qed
+   
+
+
+lemma
+ assumes base_inv:"(inv1 st0)"
+ and st1:"(st1=(setVarBool st0 ''pressure'' pressure))"
+ and st2:"(st2=(setVarBool st1 ''user'' user))"
+ and st2_Controller_state:"(getPstate st2 ''Controller'')=''motionless''"
+ and st2_if3:"(getVarBool st2 ''user'')=False"
+ and st3:"(st3=(toEnv st2))"
+ and st_final:"(st_final=st3)"
+shows "(inv1 st_final)"
+proof(simp only: inv1_def; rule conjI)
+  show "extraInv st_final" using assms extra inv1_def by auto
+next
+  show "R1 st_final"
+  proof -
+    have "toEnvP st0 \<and> toEnvP st_final \<and> st0 = predEnv st_final" using assms inv1_def extraInv_def by auto
+    moreover have "P2_predEnv R1_A2 st0" using R1_A2 assms inv1_def by auto
+    moreover have "R1_A2 st_final st0" using assms R1_A2_def by auto
+    ultimately show ?thesis using two_pos_cond_cons_exp A2_R1 by auto
+  qed
+qed
+
+
+lemma
+ assumes base_inv:"(inv2 st0)"
+ and st1:"(st1=(setVarBool st0 ''pressure'' pressure))"
+ and st2:"(st2=(setVarBool st1 ''user'' user))"
+ and st2_Controller_state:"(getPstate st2 ''Controller'')=''motionless''"
+ and st2_if3:"(getVarBool st2 ''user'')=False"
+ and st3:"(st3=(toEnv st2))"
+ and st_final:"(st_final=st3)"
+shows "(inv2 st_final)"
+proof(simp only: inv2_def; rule conjI)
+  show "extraInv st_final" using assms extra inv2_def by auto
+next
+  show "R2 st_final"
+  proof -
+    have "toEnvP st0 \<and> toEnvP st_final \<and> st0 = predEnv st_final" using assms inv2_def extraInv_def by auto
+    moreover have "P2_predEnv R2_A2 st0" using R2_A2 assms inv2_def by auto
+    moreover have "R2_A2 st_final st0" using assms R2_A2_def by auto
+    ultimately show ?thesis using two_pos_cond_cons_exp A2_R2 by auto
+  qed
+qed
+
+lemma
+ assumes base_inv:"(inv4 st0)"
+ and st1:"(st1=(setVarBool st0 ''pressure'' pressure))"
+ and st2:"(st2=(setVarBool st1 ''user'' user))"
+ and st2_Controller_state:"(getPstate st2 ''Controller'')=''motionless''"
+ and st2_if3:"(getVarBool st2 ''user'')=False"
+ and st3:"(st3=(toEnv st2))"
+ and st_final:"(st_final=st3)"
+shows "(inv4 st_final)"
+proof(simp only: inv4_def; rule conjI)
+  show "extraInv st_final" using assms extra inv4_def by auto
+next
+  show "R4 st_final"
+  proof -
+    define inv4_A1 where "inv4_A1 = P3_to_predEnv inv4_A3 st_final"
+    moreover have "toEnvP st0 \<and> toEnvP st_final \<and> st0 = predEnv st_final" using assms R4_def inv4_def by auto
+    moreover have "P3_predEnv inv4_A3 st0" using assms inv4_def inv4_A3 R4_def by auto
+    moreover have "P1 inv4_A1 st0" using assms P1_def inv4_A1_def P3_to_predEnv_def inv4_A3_def by auto
+    moreover have "inv4_A1 st_final" using assms inv4_A1_def P3_to_predEnv_def inv4_A3_def by auto
+    ultimately show ?thesis using P3_predEnv A3_inv4 by auto
+  qed
+qed
 
 end
