reflex case stadies/RevolvingDoor/RevolvingDoor_VC6.thy
@@ -2,17 +2,207 @@ theory RevolvingDoor_VC6
 imports RevolvingDoorTheory
 begin
 
-lemma
- assumes base_inv:"(inv st0)"
- and st1:"(st1=(setVarBool st0 ''inp_2'' inp_2))"
- and st2:"(st2=(setVarBool st1 ''inp_1'' inp_1))"
+
+lemma extra:
+ assumes base_inv:"(extraInv st0)"
+ and st1:"(st1=(setVarBool st0 ''pressure'' pressure))"
+ and st2:"(st2=(setVarBool st1 ''user'' user))"
  and st2_Controller_state:"(getPstate st2 ''Controller'')=''rotating''"
- and st2_if5:"(getVarBool st2 ''inp_2'')=False"
- and st2_if7:"(getVarBool st2 ''inp_1'')=False"
+ and st2_if5:"(getVarBool st2 ''pressure'')=False"
+ and st2_if7:"(getVarBool st2 ''user'')=False"
  and st2_rotating_timeout:"1000\<le>(ltime st2 ''Controller'')"
- and st3:"(st3=(setVarBool st2 ''out_1'' False))"
+ and st3:"(st3=(setVarBool st2 ''rotation'' False))"
  and st4:"(st4=(setPstate st3 ''Controller'' ''motionless''))"
  and st5:"(st5=(toEnv st4))"
-shows "(inv st5)"
+ and st_final:"(st_final=st5)"
+shows "(extraInv st_final)"
+proof (simp only: extraInv_def;intro conjI)
+  show "toEnvP st_final" using assms by auto
+next
+  show "extraControllerStates st_final"
+  proof -
+    have "extraControllerStates st0" using extraInv_def base_inv by blast
+    then show ?thesis using assms extraControllerStates_def by auto
+  qed
+next
+  show "extraMotionlessOut st_final" 
+  proof (simp only: extraMotionlessOut_def; rule allI; rule impI)
+    fix s1
+    assume prems:"toEnvP s1 \<and>
+          substate s1 st_final \<and>
+          getPstate s1 ''Controller'' = ''motionless''"
+    then show "\<not> getVarBool s1 ''rotation'' \<and>
+                \<not> getVarBool s1 ''brake''"
+    proof (cases)
+      assume 1:"s1=st_final"
+      have 2:"\<not> getVarBool st_final ''rotation''" using assms by auto
+      have "\<not> getVarBool st0 ''brake''" using assms extraInv_def extraRotatingOut_def substate_refl by auto
+      then have 3:"\<not> getVarBool st_final ''brake''" using assms by auto
+      show  ?thesis using 1 2 3  by auto
+    next
+      assume 1:"s1\<noteq>st_final"
+      have "predEnv st_final = st0" using assms extraInv_def by auto
+      then have 2:"substate s1 st0" using 1 assms prems substate_eq_or_predEnv by blast 
+      have "extraMotionlessOut st0" using base_inv extraInv_def by auto
+      thus ?thesis using 1 2 prems assms extraInv_def extraMotionlessOut_def[of st0] substate_refl by blast
+    qed
+  qed
+next
+  show "extraRotatingOut st_final" 
+  proof -
+    have "extraRotatingOut st0" using extraInv_def base_inv by blast
+    then show ?thesis using assms extraRotatingOut_def by auto
+  qed
+next
+  show "extraSuspendedOut st_final"
+  proof -
+    have "extraSuspendedOut st0" using extraInv_def base_inv by blast
+    then show ?thesis using assms extraSuspendedOut_def by auto
+  qed     
+next
+  show "extra2 st_final"
+  proof -
+    have "extra2 st0" using base_inv extraInv_def by auto
+    thus ?thesis using assms extra2_def by auto
+  qed
+next
+  show "extra3 st_final"
+  proof -
+    have "extra3 st0" using base_inv extraInv_def by auto
+    thus ?thesis using assms extra3_def by auto
+  qed
+next
+  show "extra6 st_final"
+  proof -
+    have "extra6 st0" using base_inv extraInv_def by auto
+    thus ?thesis using assms extra6_def by auto
+  qed
+next
+  show "extra4 st_final"
+  proof -
+    have "extra4 st0" using base_inv extraInv_def by auto
+    thus ?thesis using assms extra4_def by auto
+  qed
+next
+  show "extra5 st_final" 
+  proof -
+    have "extra5 st0" using base_inv extraInv_def by auto
+    thus ?thesis using assms extra5_def by auto
+  qed
+next
+  show "extra7 st_final"
+  proof -
+    have "extra7 st0" using base_inv extraInv_def by auto
+    thus ?thesis using assms extra7_def by auto
+  qed
+next
+  show "extra1 st_final"
+  proof (simp only: extra1_def; rule allI; rule impI)
+    fix s1
+    assume prems:"toEnvP s1 \<and>substate s1 st_final \<and>
+          getPstate s1 ''Controller'' = ''motionless''"
+    then show "(\<forall>s2. toEnvP s2 \<and> substate s2 s1 \<longrightarrow> getPstate s2 ''Controller'' = ''motionless'') \<or>
+          (\<exists>s2 s3.
+              toEnvP s2 \<and>
+              toEnvP s3 \<and>
+              substate s2 s3 \<and>
+              substate s3 s1 \<and>
+              toEnvNum s2 s3 = 1 \<and>
+              getPstate s2 ''Controller'' = ''rotating'' \<and>
+              1000 \<le> ltime s2 ''Controller'' \<and>
+              \<not> getVarBool s3 ''user'' \<and>
+              \<not> getVarBool s3 ''pressure'' \<and>
+              (\<forall>s4 s5.
+                  toEnvP s4 \<and>
+                  toEnvP s5 \<and> substate s3 s4 \<and> substate s4 s5 \<and> substate s5 s1 \<and> toEnvNum s4 s5 = 1 \<longrightarrow>
+                  getPstate s4 ''Controller'' = ''motionless'' \<and> \<not> getVarBool s5 ''user''))"
+    proof (cases)
+      assume 1:"s1=st_final"
+      have "toEnvP st0 \<and> 
+            toEnvP st_final" using  assms extraInv_def by auto
+      moreover have "substate st0 st_final" using assms substate_refl by auto 
+      moreover have "substate st_final s1" using 1 substate_refl by auto
+      moreover have "toEnvNum st0 st_final =1" using assms toEnvNum_id by auto
+      moreover have "getPstate st0 ''Controller'' = ''rotating''" using assms by auto
+      moreover have "1000 \<le> ltime st0 ''Controller''" using assms by auto
+      moreover have "\<not> getVarBool st_final ''user'' \<and>\<not> getVarBool st_final ''pressure''" using assms by auto
+      moreover have "(\<forall>s4 s5.
+                  toEnvP s4 \<and>
+                  toEnvP s5 \<and> substate st_final s4 \<and> substate s4 s5 \<and> substate s5 s1 \<and> toEnvNum s4 s5 = 1 \<longrightarrow>
+                  getPstate s4 ''Controller'' = ''motionless'' \<and> \<not> getVarBool s5 ''user'')" using prems 1 substate_trans substate_asym
+        using calculation(7) by blast
+      ultimately show ?thesis by auto
+    next
+      assume 1:"s1\<noteq>st_final"
+      have "predEnv st_final = st0" using assms extraInv_def by auto
+      then have 2:"substate s1 st0" using 1 assms prems substate_eq_or_predEnv by blast
+      have "extra1 st0" using assms extraInv_def by auto
+      then show ?thesis using 1 2 prems assms extraInv_def extra1_def by auto
+    qed
+  qed
+qed
 
+lemma
+ assumes base_inv:"(inv1 st0)"
+ and st1:"(st1=(setVarBool st0 ''pressure'' pressure))"
+ and st2:"(st2=(setVarBool st1 ''user'' user))"
+ and st2_Controller_state:"(getPstate st2 ''Controller'')=''rotating''"
+ and st2_if5:"(getVarBool st2 ''pressure'')=False"
+ and st2_if7:"(getVarBool st2 ''user'')=False"
+ and st2_rotating_timeout:"1000\<le>(ltime st2 ''Controller'')"
+ and st3:"(st3=(setVarBool st2 ''rotation'' False))"
+ and st4:"(st4=(setPstate st3 ''Controller'' ''motionless''))"
+ and st5:"(st5=(toEnv st4))"
+ and st_final:"(st_final=st5)"
+shows "(inv1 st_final)"
+proof(simp only: inv1_def; rule conjI)
+  show "extraInv st_final" using assms extra inv1_def by auto
+next
+  show "R1 st_final"
+  proof -
+    have "toEnvP st0 \<and> toEnvP st_final \<and> st0 = predEnv st_final" using assms inv1_def extraInv_def by auto
+    moreover have "P2_predEnv R1_A2 st0" using R1_A2 assms inv1_def by auto
+    moreover have "R1_A2 st_final st0" using assms R1_A2_def by auto
+    ultimately show ?thesis using two_pos_cond_cons_exp A2_R1 by auto
+  qed
+qed
+
+lemma
+ assumes base_inv:"(inv2 st0)"
+ and st1:"(st1=(setVarBool st0 ''pressure'' pressure))"
+ and st2:"(st2=(setVarBool st1 ''user'' user))"
+ and st2_Controller_state:"(getPstate st2 ''Controller'')=''rotating''"
+ and st2_if5:"(getVarBool st2 ''pressure'')=False"
+ and st2_if7:"(getVarBool st2 ''user'')=False"
+ and st2_rotating_timeout:"1000\<le>(ltime st2 ''Controller'')"
+ and st3:"(st3=(setVarBool st2 ''rotation'' False))"
+ and st4:"(st4=(setPstate st3 ''Controller'' ''motionless''))"
+ and st5:"(st5=(toEnv st4))"
+ and st_final:"(st_final=st5)"
+shows "(inv2 st_final)"
+proof(simp only: inv2_def; rule conjI)
+  show "extraInv st_final" using assms extra inv2_def by auto
+next
+  show "R2 st_final"
+  proof -
+    have "toEnvP st0 \<and> toEnvP st_final \<and> st0 = predEnv st_final" using assms inv2_def extraInv_def by auto
+    moreover have "P2_predEnv R2_A2 st0" using R2_A2 assms inv2_def by auto
+    moreover have "R2_A2 st_final st0" using assms R2_A2_def by auto
+    ultimately show ?thesis using two_pos_cond_cons_exp A2_R2 by auto
+  qed
+qed
+
+lemma
+ assumes base_inv:"(inv st0)"
+ and st1:"(st1=(setVarBool st0 ''pressure'' pressure))"
+ and st2:"(st2=(setVarBool st1 ''user'' user))"
+ and st2_Controller_state:"(getPstate st2 ''Controller'')=''rotating''"
+ and st2_if5:"(getVarBool st2 ''pressure'')=False"
+ and st2_if7:"(getVarBool st2 ''user'')=False"
+ and st2_rotating_timeout:"1000\<le>(ltime st2 ''Controller'')"
+ and st3:"(st3=(setVarBool st2 ''rotation'' False))"
+ and st4:"(st4=(setPstate st3 ''Controller'' ''motionless''))"
+ and st5:"(st5=(toEnv st4))"
+ and st_final:"(st_final=st5)"
+shows "(inv st_final)"
 end
