reflex case stadies/RevolvingDoor/RevolvingDoor_VC7.thy
@@ -2,15 +2,240 @@ theory RevolvingDoor_VC7
 imports RevolvingDoorTheory
 begin
 
-lemma
- assumes base_inv:"(inv st0)"
- and st1:"(st1=(setVarBool st0 ''inp_2'' inp_2))"
- and st2:"(st2=(setVarBool st1 ''inp_1'' inp_1))"
+lemma extra:
+ assumes base_inv:"(extraInv st0)"
+ and st1:"(st1=(setVarBool st0 ''pressure'' pressure))"
+ and st2:"(st2=(setVarBool st1 ''user'' user))"
  and st2_Controller_state:"(getPstate st2 ''Controller'')=''rotating''"
- and st2_if5:"(getVarBool st2 ''inp_2'')=False"
- and st2_if7:"(getVarBool st2 ''inp_1'')=False"
+ and st2_if5:"(getVarBool st2 ''pressure'')=False"
+ and st2_if7:"(getVarBool st2 ''user'')=False"
  and st2_rotating_timeout:"1000>(ltime st2 ''Controller'')"
  and st3:"(st3=(toEnv st2))"
-shows "(inv st3)"
+ and st_final:"(st_final=st3)"
+shows "(extraInv st_final)"
+proof (simp only: extraInv_def;intro conjI)
+  show "toEnvP st_final" using assms by auto
+next
+  show "extraControllerStates st_final"
+  proof -
+    have "extraControllerStates st0" using extraInv_def base_inv by blast
+    then show ?thesis using assms extraControllerStates_def by auto
+  qed
+next
+  show "extraMotionlessOut st_final" 
+  proof -
+    have "extraMotionlessOut st0" using extraInv_def base_inv by blast
+    then show ?thesis using assms extraMotionlessOut_def by auto
+  qed
+next
+  show "extraRotatingOut st_final" 
+  proof (simp only:extraRotatingOut_def; rule allI; rule impI)
+    fix s1
+    assume prems:"toEnvP s1 \<and>
+          substate s1 st_final \<and>
+          getPstate s1 ''Controller'' = ''rotating''"
+    then show "getVarBool s1 ''rotation'' \<and>
+          \<not> getVarBool s1 ''brake'' \<and>
+          ltime s1 ''Controller'' \<le> 1000"
+    proof (cases)
+      assume 1:"s1=st_final"
+      have "\<not> getVarBool st0 ''brake''" using extraRotatingOut_def substate_refl assms extraInv_def by auto
+      then have 2:"\<not> getVarBool st_final ''brake''" using assms by auto
+      have 3: "getVarBool st_final ''rotation''" using extraRotatingOut_def substate_refl assms extraInv_def by auto
+      have "1000=(10*100::nat) \<and> 900=(10*100::nat) -100" by auto
+      then have "(ltime st2 ''Controller'')\<le>900" using assms ltime_mod by presburger
+      then have 4: "ltime st_final ''Controller'' \<le> 1000" using assms ltime_div_less  by auto
+      show ?thesis using 1 2 3 4 by auto
+    next
+      assume 1:"s1\<noteq>st_final"
+      have "predEnv st_final = st0" using assms extraInv_def by auto
+      then have 2:"substate s1 st0" using 1 assms prems substate_eq_or_predEnv by blast
+      have "extraRotatingOut st0" using base_inv extraInv_def by auto
+      thus ?thesis using 1 2 prems assms extraInv_def extraRotatingOut_def by auto
+    qed
+  qed
+next
+  show "extraSuspendedOut st_final"
+  proof -
+    have "extraSuspendedOut st0" using extraInv_def base_inv by blast
+    then show ?thesis using assms extraSuspendedOut_def by auto
+  qed
+next
+  show "extra1 st_final"
+  proof -
+    have "extra1 st0" using base_inv extraInv_def by auto
+    thus ?thesis using assms extra1_def by auto
+  qed
+next
+  show "extra2 st_final"
+  proof (simp only: extra2_def; rule allI; rule impI)
+    fix s1
+    assume prems:"toEnvP s1 \<and>
+                  substate s1 st_final \<and>
+                  getPstate s1 ''Controller'' = ''rotating''"
+    thus "\<exists>s2 s3.
+             toEnvP s2 \<and>
+             toEnvP s3 \<and>
+             substate s2 s3 \<and>
+             substate s3 s1 \<and>
+             toEnvNum s2 s3 = 1 \<and>
+             toEnvNum s2 s1 = ltime s1 ''Controller'' div 100 \<and>
+             ((getPstate s2 ''Controller'' = ''motionless'' \<or>
+               getPstate s2 ''Controller'' = ''rotating'') \<and>
+              getVarBool s3 ''user'' \<or>
+              getPstate s2 ''Controller'' = ''suspended'') \<and>
+             \<not> getVarBool s3 ''pressure''"
+    proof (cases)
+      assume 1:"s1=st_final"
+      have 2:"extra2 st0" using assms extraInv_def by auto
+      have 3:"substate st0 st_final" using assms substate_refl by auto
+      show ?thesis using 1 2 3 assms extraInv_def extra2_def by sorry
+    next
+      assume 1:"s1\<noteq>st_final"
+      have "predEnv st_final = st0" using assms extraInv_def by auto
+      then have 2:"substate s1 st0" using 1 assms prems substate_eq_or_predEnv by blast
+      have "extra2 st0" using assms extraInv_def by auto
+      then show ?thesis using 1 2 prems assms extraInv_def extra2_def by auto
+    qed
+  qed
+next
+  show "extra3 st_final"
+  proof (simp only:extra3_def; rule allI; rule impI)
+    fix s1
+    assume prems:"toEnvP s1 \<and>
+            substate s1 st_final \<and>
+            getPstate s1 ''Controller'' = ''rotating''"
+    then show "\<exists>s2 s3.
+             toEnvP s2 \<and>
+             toEnvP s3 \<and>
+             substate s2 s3 \<and>
+             substate s3 s1 \<and>
+             toEnvNum s2 s3 = 1 \<and>
+             (getPstate s2 ''Controller'' = ''motionless'' \<and>
+              getVarBool s3 ''user'' \<or>
+              getPstate s2 ''Controller'' = ''suspended'') \<and>
+             \<not> getVarBool s3 ''pressure'' \<and>
+             (\<forall>s4. toEnvP s4 \<and> substate s3 s4 \<and> substate s4 s1 \<longrightarrow>
+                   getPstate s4 ''Controller'' = ''rotating'')"
+    proof - 
+      have "extra3 st0" using assms extraInv_def by auto
+      then obtain 1:"(\<forall> s1. 
+                toEnvP s1 \<and> 
+                substate s1 st0 \<and> 
+                getPstate s1 ''Controller'' = ''rotating'' \<longrightarrow>
+                  (\<exists> s2 s3. 
+                    toEnvP s2 \<and> 
+                    toEnvP s3 \<and> 
+                    substate s2 s3 \<and> 
+                    substate s3 s1 \<and> 
+                    toEnvNum s2 s3 = 1 \<and> 
+                    (getPstate s2 ''Controller'' = ''motionless'' \<and> 
+                      getVarBool s3 ''user'' \<or>
+                      getPstate s2 ''Controller'' = ''suspended'') \<and> 
+                    \<not> getVarBool s3 ''pressure'' \<and>
+                    (\<forall> s4. 
+                      toEnvP s4 \<and> 
+                      substate s3 s4 \<and> 
+                      substate s4 s1 \<longrightarrow> 
+                        getPstate s4 ''Controller'' = ''rotating'')))" using extra3_def by auto
+      have 2:"substate st0 st_final" using assms substate_refl by auto
+      then show ?thesis using 1 assms prems extraInv_def extra3_def substate_refl substate_trans by sorry
+    qed
+  qed
+next
+  show "extra6 st_final"
+  proof -
+    define ex6_A1 where "ex6_A1 = P3_to_predEnv ex6_A3 st_final"
+    moreover have "toEnvP st0 \<and> toEnvP st_final \<and> st0 = predEnv st_final" using assms extraInv_def by auto
+    moreover have "P3_predEnv ex6_A3 st0" using assms extraInv_def ex6_A3 by auto
+    moreover have "ex6_A1 st_final" 
+    proof -
+      have "getPstate st0 ''Controller'' = ''rotating''" using assms by auto
+      moreover have "\<not>getVarBool st_final ''user''" using assms by auto
+      ultimately show  "ex6_A1 st_final" using ex6_A1_def P3_to_predEnv_def ex6_A3_def assms extraInv_def by auto
+    qed
+    moreover have "P1 ex6_A1 st0"  by sorry
+    ultimately show ?thesis using A3_ex6_sub P3_cons_from_predEnv P3_predEnv by blast 
+  qed
+next
+  show "extra4 st_final"
+  proof -
+    have "extra4 st0" using base_inv extraInv_def by auto
+    thus ?thesis using assms extra4_def by auto
+  qed
+next
+  show "extra5 st_final" 
+  proof -
+    have "extra5 st0" using base_inv extraInv_def by auto
+    thus ?thesis using assms extra5_def by auto
+  qed
+next
+  show "extra7 st_final"
+  proof -
+    have "extra7 st0" using base_inv extraInv_def by auto
+    thus ?thesis using assms extra7_def by auto
+  qed
+qed
+
+
+
+lemma
+ assumes base_inv:"(inv1 st0)"
+ and st1:"(st1=(setVarBool st0 ''pressure'' pressure))"
+ and st2:"(st2=(setVarBool st1 ''user'' user))"
+ and st2_Controller_state:"(getPstate st2 ''Controller'')=''rotating''"
+ and st2_if5:"(getVarBool st2 ''pressure'')=False"
+ and st2_if7:"(getVarBool st2 ''user'')=False"
+ and st2_rotating_timeout:"1000>(ltime st2 ''Controller'')"
+ and st3:"(st3=(toEnv st2))"
+ and st_final:"(st_final=st3)"
+shows "(inv1 st_final)"
+proof(simp only: inv1_def; rule conjI)
+  show "extraInv st_final" using assms extra inv1_def by auto
+next
+  show "R1 st_final"
+  proof -
+    have "toEnvP st0 \<and> toEnvP st_final \<and> st0 = predEnv st_final" using assms inv1_def extraInv_def by auto
+    moreover have "P2_predEnv R1_A2 st0" using R1_A2 assms inv1_def by auto
+    moreover have "R1_A2 st_final st0" using assms R1_A2_def by auto
+    ultimately show ?thesis using two_pos_cond_cons_exp A2_R1 by auto
+  qed
+qed
+
+
+lemma
+ assumes base_inv:"(inv2 st0)"
+ and st1:"(st1=(setVarBool st0 ''pressure'' pressure))"
+ and st2:"(st2=(setVarBool st1 ''user'' user))"
+ and st2_Controller_state:"(getPstate st2 ''Controller'')=''rotating''"
+ and st2_if5:"(getVarBool st2 ''pressure'')=False"
+ and st2_if7:"(getVarBool st2 ''user'')=False"
+ and st2_rotating_timeout:"1000>(ltime st2 ''Controller'')"
+ and st3:"(st3=(toEnv st2))"
+ and st_final:"(st_final=st3)"
+shows "(inv2 st_final)"
+proof(simp only: inv2_def; rule conjI)
+  show "extraInv st_final" using assms extra inv2_def by auto
+next
+  show "R2 st_final"
+  proof -
+    have "toEnvP st0 \<and> toEnvP st_final \<and> st0 = predEnv st_final" using assms inv2_def extraInv_def by auto
+    moreover have "P2_predEnv R2_A2 st0" using R2_A2 assms inv2_def by auto
+    moreover have "R2_A2 st_final st0" using assms R2_A2_def by auto
+    ultimately show ?thesis using two_pos_cond_cons_exp A2_R2 by auto
+  qed
+qed
+
+lemma
+ assumes base_inv:"(inv st0)"
+ and st1:"(st1=(setVarBool st0 ''pressure'' pressure))"
+ and st2:"(st2=(setVarBool st1 ''user'' user))"
+ and st2_Controller_state:"(getPstate st2 ''Controller'')=''rotating''"
+ and st2_if5:"(getVarBool st2 ''pressure'')=False"
+ and st2_if7:"(getVarBool st2 ''user'')=False"
+ and st2_rotating_timeout:"1000>(ltime st2 ''Controller'')"
+ and st3:"(st3=(toEnv st2))"
+ and st_final:"(st_final=st3)"
+shows "(inv st_final)"
 
 end
