reflex case stadies/RevolvingDoor/buff/RevolvingDoor_VC10.thy
@@ -1,0 +1,16 @@
+theory RevolvingDoor_VC10
+imports RevolvingDoorTheory
+begin
+
+lemma
+ assumes base_inv:"(inv st0)"
+ and st1:"(st1=(setVarBool st0 ''pressure'' pressure))"
+ and st2:"(st2=(setVarBool st1 ''user'' user))"
+ and st2_Controller_state:"(getPstate st2 ''Controller'')=''suspended''"
+ and st2_if9:"(getVarBool st2 ''pressure'')=False"
+ and st2_suspended_timeout:"1000>(ltime st2 ''Controller'')"
+ and st3:"(st3=(toEnv st2))"
+ and st_final:"(st_final=st3)"
+shows "(inv st_final)"
+
+end
