reflex case stadies/Thermopot/-Thermopot_VC89.thy
@@ -1,0 +1,21 @@
+theory Thermopot_VC89
+imports ThermopotTheory
+begin
+
+lemma
+ assumes base_inv:"(inv st0)"
+ and st1:"(st1=(setVarBool st0 ''buttons_1'' buttons_1))"
+ and st2:"(st2=(setVarInt st1 ''temperature_0'' temperature_0))"
+ and st3:"(st3=(setVarBool st2 ''buttons_2'' buttons_2))"
+ and st4:"(st4=(setVarBool st3 ''buttons_3'' buttons_3))"
+ and st5:"(st5=(setVarBool st4 ''boilingButton_0'' boilingButton_0))"
+ and st5_Init_state:"(getPstate st5 ''Init'')=''stop''"
+ and st5_TempSelection_state:"(getPstate st5 ''TempSelection'')=''stop''"
+ and st5_HeaterController_state:"(getPstate st5 ''HeaterController'')=''maintaining''"
+ and st5_if17:"((getVarBool st5 ''boilingButton_0'') = True)=False"
+ and st5_if19:"((getVarInt st5 ''temperature_0'') \<ge> (getVarInt st5 ''selectedTemp_0''))=False"
+ and st5_if21:"((getVarInt st5 ''temperature_0'') < ((getVarInt st5 ''selectedTemp_0'') - 5))=False"
+ and st6:"(st6=(toEnv st5))"
+shows "(inv st6)"
+
+end
