reflex case stadies/Thermopot/Thermopot_VC28.thy
@@ -1,0 +1,27 @@
+theory Thermopot_VC28
+imports ThermopotTheory
+begin
+
+lemma
+ assumes base_inv:"(inv st0)"
+ and st1:"(st1=(setVarBool st0 ''buttons_1'' buttons_1))"
+ and st2:"(st2=(setVarInt st1 ''temperature_0'' temperature_0))"
+ and st3:"(st3=(setVarBool st2 ''buttons_2'' buttons_2))"
+ and st4:"(st4=(setVarBool st3 ''buttons_3'' buttons_3))"
+ and st5:"(st5=(setVarBool st4 ''boilingButton_0'' boilingButton_0))"
+ and st5_Init_state:"(getPstate st5 ''Init'')=''begin''"
+ and st6:"(st6=(setPstate st5 ''TempSelection'' ''tempSelection''))"
+ and st7:"(st7=(setPstate st6 ''HeaterController'' ''begin''))"
+ and st8:"(st8=(setPstate st7 ''Init'' ''''stop''''))"
+ and st8_TempSelection_state:"(getPstate st8 ''TempSelection'')=''tempSelection''"
+ and st8_if1:"((getVarBool st8 ''buttons_1'') = True)=False"
+ and st8_if3:"((getVarBool st8 ''buttons_2'') = True)=False"
+ and st8_if5:"((getVarBool st8 ''buttons_3'') = True)=False"
+ and st8_HeaterController_state:"(getPstate st8 ''HeaterController'')=''begin''"
+ and st8_if6:"((getVarBool st8 ''boilingButton_0'') = True)=True"
+ and st9:"(st9=(setVarBool st8 ''mods_0'' True))"
+ and st10:"(st10=(setPstate st9 ''HeaterController'' ''heating''))"
+ and st11:"(st11=(toEnv st10))"
+shows "(inv st11)"
+
+end
