reflex case stadies/Thermopot/Thermopot_VC70.thy
@@ -1,0 +1,26 @@
+theory Thermopot_VC70
+imports ThermopotTheory
+begin
+
+lemma
+ assumes base_inv:"(inv st0)"
+ and st1:"(st1=(setVarBool st0 ''buttons_1'' buttons_1))"
+ and st2:"(st2=(setVarInt st1 ''temperature_0'' temperature_0))"
+ and st3:"(st3=(setVarBool st2 ''buttons_2'' buttons_2))"
+ and st4:"(st4=(setVarBool st3 ''buttons_3'' buttons_3))"
+ and st5:"(st5=(setVarBool st4 ''boilingButton_0'' boilingButton_0))"
+ and st5_Init_state:"(getPstate st5 ''Init'')=''stop''"
+ and st5_TempSelection_state:"(getPstate st5 ''TempSelection'')=''tempSelection''"
+ and st5_if1:"((getVarBool st5 ''buttons_1'') = True)=False"
+ and st5_if3:"((getVarBool st5 ''buttons_2'') = True)=False"
+ and st5_if4:"((getVarBool st5 ''buttons_3'') = True)=True"
+ and st6:"(st6=(setVarInt st5 ''selectedTemp_0'' 60))"
+ and st6_HeaterController_state:"(getPstate st6 ''HeaterController'')=''maintaining''"
+ and st6_if19:"((getVarBool st6 ''boilingButton_0'') = True)=False"
+ and st6_if21:"((getVarInt st6 ''temperature_0'') \<ge> (getVarInt st6 ''selectedTemp_0''))=False"
+ and st6_if22:"((getVarInt st6 ''temperature_0'') < ((getVarInt st6 ''selectedTemp_0'') - 5))=True"
+ and st7:"(st7=(setVarBool st6 ''heater_0'' True))"
+ and st8:"(st8=(toEnv st7))"
+shows "(inv st8)"
+
+end
