reflex case stadies/RevolvingDoor/RevolvingDoor_VC0.thy~
@@ -1,0 +1,12 @@
+theory RevolvingDoor_VC0
+imports RevolvingDoorTheory
+begin
+
+lemma
+ assumes st0:"(st0=emptyState)"
+ and st1:"(st1=(setPstate st0 ''Controller'' ''motionless''))"
+ and st2:"(st2=(toEnv st1))"
+ and st_final:"(st_final=st2)"
+shows "(inv st_final)"
+
+end
